widen

InferApp.v
@@ -1,10 +1,15 @@
-Require Export SystemFR.ScalaDepSugar.
 Require Export SystemFR.ErasedArrow.
+Require Export SystemFR.ErasedSingleton.
 Require Export SystemFR.ReducibilitySubtype.
+
+Opaque reducible_values.
 
 Inductive widen: tree -> tree -> Prop :=
 | WidenSingleton:
     forall ty1 ty2 f,
+      is_erased_term f ->
+      is_erased_type ty2 ->
+      wf f 0 ->
       widen
         (T_singleton (T_arrow ty1 ty2) f)
         (T_arrow ty1 (T_singleton ty2 (app f (lvar 0 term_var))))
@@ -16,14 +21,57 @@ Inductive widen: tree -> tree -> Prop :=
     forall ty, widen ty ty
 .
 
+Lemma reducible_equiv:
+  forall ρ t1 t2,
+    [ t1 ≡ t2 ] ->
+    [ ρ | uu : T_equiv t1 t2 ].
+Proof.
+  intros; unfold reducible, reduces_to; repeat step || exists uu || simp_red; t_closer.
+Qed.
+
+Lemma widen_singleton_arrow:
+  forall Θ Γ ty1 ty2 f,
+    is_erased_term f ->
+    is_erased_type ty2 ->
+    wf f 0 ->
+    [Θ; Γ ⊨ T_singleton (T_arrow ty1 ty2) f <:
+            T_arrow ty1 (T_singleton ty2 (app f (lvar 0 term_var))) ].
+Proof.
+  unfold open_subtype, subtype;
+    repeat step || simp_red || open_none || apply reducible_type_refine with uu ||
+           (rewrite shift_nothing2 in * by eauto with wf) || list_utils ||
+           apply reducible_equiv || t_instantiate_reducible ||
+           apply equivalent_app ||
+           rewrite reducibility_rewrite in *;
+    eauto with wf fv erased;
+    eauto using reducible_values_closed;
+    try solve [ apply equivalent_refl; eauto with wf fv erased ].
+Qed.
+
+Lemma singleton_subtype:
+  forall Θ Γ ty f,
+    [ Θ; Γ ⊨ T_singleton ty f <: ty ].
+Proof.
+  unfold open_subtype, subtype; repeat step || simp_red.
+Qed.
+
+Lemma widen_singleton:
+  forall Θ Γ ty ty' f,
+    [Θ; Γ ⊨ ty <: ty'] ->
+    [Θ; Γ ⊨ T_singleton ty f <: ty'].
+Proof.
+  eauto using open_subtype_trans, singleton_subtype.
+Qed.
+
 Lemma widen_open_subtype:
   forall Θ Γ ty1 ty2,
     widen ty1 ty2 ->
     [ Θ; Γ ⊨ ty1 <: ty2 ].
 Proof.
-  induction 1;
-    repeat step.
-Admitted.
+  induction 1; repeat step;
+    eauto using widen_singleton_arrow;
+    eauto using widen_singleton.
+Qed.
 
 Lemma open_tapp_helper:
   forall Θ Γ t1 t2 S T U,
